EasyCrypt/Array19200.ec
@@ -1,3 +1,0 @@
-from Jasmin require import JArray.
-
-clone export PolyArray as Array19200  with op size <- 19200.
